Strata/Transform/DetToNondet.lean
@@ -16,7 +16,7 @@ mutual
 
 /-- Deterministic-to-nondeterministic transformation for a single
 (deterministic) statement -/
-def StmtToNondetStmt {P : PureExpr} [Imperative.HasBool P] [Imperative.HasBoolNeg P]
+def StmtToNondetStmt {P : PureExpr} [Imperative.HasBool P] [HasNot P]
   (st : Imperative.Stmt P (Cmd P)) :
   Imperative.NondetStmt P (Cmd P) :=
   match st with
@@ -25,14 +25,14 @@ def StmtToNondetStmt {P : PureExpr} [Imperative.HasBool P] [Imperative.HasBoolNe
   | .ite    cond ⟨ tss ⟩ ⟨ ess ⟩ md =>
     .choice
       (.seq (.assume "true_cond" cond md) (StmtsToNondetStmt tss))
-      (.seq ((.assume "false_cond" (Imperative.HasBoolNeg.neg cond) md)) (StmtsToNondetStmt ess))
+      (.seq ((.assume "false_cond" (Imperative.HasNot.not cond) md)) (StmtsToNondetStmt ess))
   | .loop   guard _measure _inv ⟨ bss ⟩ md =>
     .loop (.seq (.assume "guard" guard md) (StmtsToNondetStmt bss))
   | .goto _ _ => (.assume "skip" Imperative.HasBool.tt)
 
 /-- Deterministic-to-nondeterministic transformation for multiple
 (deterministic) statements -/
-def StmtsToNondetStmt {P : Imperative.PureExpr} [Imperative.HasBool P] [Imperative.HasBoolNeg P]
+def StmtsToNondetStmt {P : Imperative.PureExpr} [Imperative.HasBool P] [HasNot P]
   (ss : Imperative.Stmts P (Cmd P)) :
   Imperative.NondetStmt P (Cmd P) :=
   match ss with
