Strata/Transform/LoopElim.lean
@@ -4,65 +4,77 @@
   SPDX-License-Identifier: Apache-2.0 OR MIT
 -/
 
-import Strata.DL.Lambda.LExpr
-import Strata.Languages.Boogie.Statement
+import Strata.DL.Imperative.Stmt
 
 namespace Boogie
 open Imperative Lambda
 
 /-! ## Loop elimination
 
-This transformation recursively removes loops from a Boogie statement, resulting
-in a new, acyclic statement. If a loop invariant is present, it adds checks that
-the invariant is established on entry and re-established at the end of each
-iteration.
+This transformation recursively removes loops from a statement, resulting in a
+new, acyclic statement. If a loop invariant is present, it adds checks that the
+invariant is established on entry and re-established at the end of each
+iteration. If a loop invariant is not present, this transformation isn't very
+useful.
 
 -/
 
-partial
-def Statement.removeLoopsM (s : Boogie.Statement) : StateM Nat Boogie.Statement :=
-  let incState : StateM Nat Unit := StateT.modifyGet (fun x => ((), x + 1))
+mutual
+
+def Stmt.removeLoopsM
+  [HasNot P] [HasVarsImp P C] [HasHavoc P C] [HasPassiveCmds P C]
+  (s : Stmt P C) : StateM Nat (Stmt P C) :=
   match s with
-  | .loop guard _ invariant? body _ => do
-    let invariant := invariant?.getD LExpr.true
-    let loop_num ← StateT.get
-    let neg_guard : Expression.Expr := .app boolNotOp guard
-    let assigned_vars := (Stmts.modifiedVars body.ss).map (λ s => s.name)
-    let havocd : Statement :=
+  | .loop guard _ invariant? ⟨ bss ⟩ _ => do
+    let invariant := invariant?.getD HasBool.tt
+    let loop_num ← StateT.modifyGet (fun x => (x, x + 1))
+    let neg_guard : P.Expr := HasNot.not guard
+    let assigned_vars := Stmts.modifiedVars bss
+    let havocd : Stmt P C :=
       .block s!"loop_havoc_{loop_num}" {
-        ss := assigned_vars.map (λ n => Statement.havoc (Coe.coe n) {})
+        ss := assigned_vars.map (λ n => Stmt.cmd (HasHavoc.havoc n))
       } {}
-    let entry_invariant : Statement :=
-      .assert s!"entry_invariant_{loop_num}" invariant {}
-    let first_iter_facts : Statement :=
+    let entry_invariant :=
+      Stmt.cmd (HasPassiveCmds.assert s!"entry_invariant_{loop_num}" invariant)
+    let first_iter_facts :=
       .block s!"first_iter_asserts_{loop_num}" {ss := [entry_invariant]} {}
     let arbitrary_iter_assumes := .block s!"arbitrary_iter_assumes_{loop_num}" {
-      ss := [(Statement.assume s!"assume_guard_{loop_num}" guard {}),
-             (Statement.assume s!"assume_invariant_{loop_num}" invariant {})]}
-    let maintain_invariant : Statement :=
-      .assert s!"arbitrary_iter_maintain_invariant_{loop_num}" invariant {}
-    incState
-    let body_statements ← body.ss.mapM removeLoopsM
-    let arbitrary_iter_facts : Statement := .block s!"arbitrary_iter_facts_{loop_num}" {
+      ss := [(Stmt.cmd (HasPassiveCmds.assume s!"assume_guard_{loop_num}" guard)),
+             (Stmt.cmd (HasPassiveCmds.assume s!"assume_invariant_{loop_num}" invariant))]}
+    let maintain_invariant :=
+      Stmt.cmd (HasPassiveCmds.assert s!"arbitrary_iter_maintain_invariant_{loop_num}" invariant)
+    let body_statements ← Stmts.removeLoopsM bss
+    let arbitrary_iter_facts := .block s!"arbitrary_iter_facts_{loop_num}" {
       ss := [havocd, arbitrary_iter_assumes] ++
             body_statements ++
             [maintain_invariant]
     } {}
-    let not_guard : Statement := .assume s!"not_guard_{loop_num}" neg_guard {}
-    let invariant : Statement := .assume s!"invariant_{loop_num}" invariant {}
+    let not_guard := Stmt.cmd (HasPassiveCmds.assume s!"not_guard_{loop_num}" neg_guard)
+    let invariant := Stmt.cmd (HasPassiveCmds.assume s!"invariant_{loop_num}" invariant)
     pure (.ite guard {ss := [first_iter_facts, arbitrary_iter_facts, havocd, not_guard, invariant]} { ss := [] } {})
-  | .ite c t e md => do
-    incState
-    let tss ← t.ss.mapM removeLoopsM
-    incState
-    let ess ← e.ss.mapM removeLoopsM
+  | .ite c ⟨ tss ⟩ ⟨ ess ⟩ md => do
+    let tss ← Stmts.removeLoopsM tss
+    let ess ← Stmts.removeLoopsM ess
     pure (.ite c { ss := tss } { ss := ess } md)
-  | .block label b md => do
-    incState
-    let bss ← b.ss.mapM removeLoopsM
+  | .block label ⟨ bss ⟩ md => do
+    let bss ← Stmts.removeLoopsM bss
     pure (.block label { ss := bss } md)
   | .cmd _ => pure s
   | .goto _ _ => pure s
 
-def Statement.removeLoops (s : Boogie.Statement) : Boogie.Statement :=
+def Stmts.removeLoopsM
+  [HasNot P] [HasVarsImp P C] [HasHavoc P C] [HasPassiveCmds P C]
+  (ss : List (Stmt P C)) : StateM Nat (List (Stmt P C)) :=
+  match ss with
+  | [] => pure []
+  | s :: ss => do
+    let s ← Stmt.removeLoopsM s
+    let ss ← Stmts.removeLoopsM ss
+    pure (s :: ss)
+
+end
+
+def Stmt.removeLoops
+  [HasNot P] [HasVarsImp P C] [HasHavoc P C] [HasPassiveCmds P C]
+  (s : Stmt P C) : Stmt P C :=
   (StateT.run (removeLoopsM s) 0).fst
